several updates

Parametricity.v
@@ -1,54 +1,141 @@
-Require Import List Arith.
-Require MSets FMapAVL.
+Require Import
+  Coq.FSets.FMapAVL
+  Coq.FSets.FMapFacts
+  Coq.Structures.OrderedTypeEx
+  Coq.Logic.FunctionalExtensionality.
 
-Module S := Coq.MSets.MSetAVL.Make Coq.Structures.OrdersEx.Nat_as_OT.
-Module M := Coq.FSets.FMapAVL.Make Coq.Structures.OrderedTypeEx.Nat_as_OT.
 
-Inductive type: Type :=
-| Bool    :                 type
-| Nat     :                 type
-| Var     : nat  ->         type
-| Prod    : type -> type -> type
-| List    : type         -> type
-| Lambda  : type -> type -> type
-| Forall  : nat  -> type -> type
-.
 
-Fixpoint type2Type(t: type)(x: M.t Type): Type :=
+Module M := FMapAVL.Make Nat_as_OT.
+
+Module P := WProperties_fun Nat_as_OT M.
+Module F := P.F.
+
+Inductive type: Set :=
+  | Bool    :                 type
+  | Nat     :                 type
+  | Var     : nat  ->         type
+  | Prod    : type -> type -> type
+(*| List    : type         -> type*)
+  | Lambda  : type -> type -> type
+  | Forall  : nat  -> type -> type
+  .
+
+
+Definition update{V} k v (env: nat -> V) k': V :=
+  if Nat.eqb k k' then v else env k'.
+
+
+Fixpoint type2Type(t: type)(env: nat -> Type): Type :=
   match t with 
   | Bool => bool
   | Nat => nat
-  | Var n => match M.find n x with Some T => T | None => Empty_set end
-  | Prod t1 t2 => prod (type2Type t1 x) (type2Type t2 x)
-  | List t => list (type2Type t x)
-  | Lambda t1 t2 => (type2Type t1 x) -> (type2Type t2 x)
-  | Forall v t => forall (tt: Type), (type2Type t (M.add v tt x))
+  | Var v => env v
+  | Prod t1 t2 => prod (type2Type t1 env) (type2Type t2 env)
+(*| List t => list (type2Type t env) *)
+  | Lambda t1 t2 => (type2Type t1 env) -> (type2Type t2 env)
+  | Forall v t => forall (tt: Type), (type2Type t (update v tt env))
   end.
 
 
-Definition x := type2Type (Prod Bool Nat) (M.empty _).
+Definition x := type2Type (Prod Bool Nat) (fun _ => Empty_set).
 Definition y: x := pair true 4.
 
 
 Inductive Rel := Rel_ A A' (R: A -> A' -> Prop).
 
-Definition p1(R: Rel): Type := match R with Rel_ T _ _ => T end.
-Definition p2(R: Rel): Type := match R with Rel_ _ T _ => T end.
+Definition p1 (env: nat -> Rel) n: Type := match env n with Rel_ T _ _ => T end.
+Definition p2 (env: nat -> Rel) n: Type := match env n with Rel_ _ T _ => T end.
+Definition rel(env: nat -> Rel) n: p1 env n -> p2 env n -> Prop :=
+  match env n as R
+    return match R with Rel_ A _ _ => A end -> match R with Rel_ _ A _ => A end -> Prop 
+    with Rel_ _ _ R => R end.
 
+Lemma p1_update{A A'} k R env: update k A (p1 env) = p1 (update k (Rel_ A A' R) env).
+Proof.
+  unfold update, p1.
+  extensionality k'.
+  destruct (Nat.eqb k k'); reflexivity.
+Qed.
 
-Fixpoint type2Rel(t: type)(Rs: M.t Rel): type2Type t (M.map p1 Rs) -> type2Type t (M.map p2 Rs) -> Prop :=
+Lemma p2_update{A A'} k R env: update k A' (p2 env) = p2 (update k (Rel_ A A' R) env).
+Proof.
+  unfold update, p2.
+  extensionality k'.
+  destruct (Nat.eqb k k'); reflexivity.
+Qed.
+
+Definition lift1{k t' A A' R env}(x: type2Type t' (update k A (p1 env))):
+                                     type2Type t' (p1 (update k (Rel_ A A' R) env)).
+  rewrite <- p1_update.
+  assumption.
+Defined.
+
+Definition lift2{k t' A A' R env}(x: type2Type t' (update k A' (p2 env))):
+                                     type2Type t' (p2 (update k (Rel_ A A' R) env)).
+  rewrite <- p2_update.
+  assumption.
+Defined.
+
+Fixpoint type2Rel(t: type)(env: nat -> Rel): type2Type t (p1 env) -> type2Type t (p2 env) -> Prop :=
   match t with 
   | Bool => eq
   | Nat => eq
-  | Var n => match M.find n Rs with Some (Rel_ A A' R) => _ | None => fun _ _ => False end
+  | Var v => rel env v
   | Prod t1 t2 => fun v1 v2 =>
     match v1, v2 with
-     (v1a, v1b), (v2a, v2b) => type2Rel _ Rs v1a v2a /\ type2Rel _ Rs v1b v2b
+     (v1a, v1b), (v2a, v2b) => type2Rel _ env v1a v2a /\ type2Rel _ env v1b v2b
     end
-  | List t => fun v1 v2 => False
+(*| List t => fun v1 v2 => False*)
   | Lambda t1 t2 => fun f1 f2 =>
-    forall v1 v2, type2Rel _ Rs v1 v2 -> type2Rel _ Rs (f1 v1) (f2 v2)
-  | Forall X F => fun g g' =>
-    forall A A' (R: A -> A' -> Prop) a a', R a a' -> type2Rel _ (M.add X (Rel_ _ _ R) Rs) (g A) (g' A')
+    forall v1 v2, type2Rel _ env v1 v2 -> type2Rel _ env (f1 v1) (f2 v2)
+  | Forall X t' => fun g g' =>
+      forall A A' (R: A -> A' -> Prop),
+        type2Rel t' (update X (Rel_ _ _ R) env) (lift1 (g A)) (lift2 (g' A'))
   end.
+
+
+Definition type2Type'(T: type): Type :=
+  type2Type T (fun _ => Empty_set).
+
+Definition type2Rel' (T: type): type2Type' T -> type2Type' T -> Prop :=
+  type2Rel T (fun _ => Rel_ Empty_set Empty_set (fun _ _ => False)).
+
+
+
+Theorem Parametricity: forall T (t: type2Type' T), type2Rel' T t t.
+Proof.
+  unfold type2Type', type2Rel'.
+  induction T; simpl; try auto.
+  intros [].
+  intros [t1 t2]. auto.
+  set (R1 := type2Rel T1 (fun _ : nat => Rel_ Empty_set Empty_set (fun _ _ : Empty_set => False))) in * |- *.
+  set (R2 := type2Rel T2 (fun _ : nat => Rel_ Empty_set Empty_set (fun _ _ : Empty_set => False))) in * |- *.
+  unfold p1, p2 in * |- *.
+  set (TT1 := type2Type T1 (fun _ : nat => Empty_set)) in * |- *.
+  set (TT2 := type2Type T2 (fun _ : nat => Empty_set)) in * |- *.
+  intros f a1 a2 H.
+
+Qed.
+
+
+
+Definition I : type := Forall 0 (Lambda (Var 0) (Var 0)).
+Definition It: Type := type2Type I (fun _ => Empty_set).
+Definition Ir: It -> It -> Prop := type2Rel I (fun _ => Rel_ Empty_set Empty_set (fun _ _ => False)).
+
+Definition i: It := fun X (x: X) => x.
+
+Theorem foo: Ir i i.
+Proof.
+  unfold Ir.
+  compute.
+  intros A A' R a a' H.
+  apply H.
+  set (H3 := p1_update 0 R (fun _ : nat => Rel_ Empty_set Empty_set (fun _ _ : Empty_set => False))).
+  set (H4 := p2_update 0 R (fun _ : nat => Rel_ Empty_set Empty_set (fun _ _ : Empty_set => False))).
+  generalize H3.
+
+
+ simpl.
 
